Refinery/Term/Extrinsic/Semantics/Effect.lean
@@ -1,0 +1,35 @@
+import Refinery.Term.Extrinsic.Semantics.Typing
+import Refinery.Term.Extrinsic.Effect
+
+namespace Refinery
+
+open CategoryTheory
+
+open MonoidalCategory' PremonoidalCategory DistributiveCategory
+
+open scoped MonoidalCategory
+
+open ChosenFiniteCoproducts
+
+variable {φ : Type _} {α : outParam (Type _)} {ε : outParam (Type _)} [S : Signature φ α ε]
+         {C : Type _} [Category C] [PremonoidalCategory C] [CC : ChosenFiniteCoproducts C]
+        [BraidedCategory' C] [Iterate C] [E : Elgot2 C ε] [Model φ α ε C]
+
+namespace Term
+
+instance Deriv.instHasEff {e : ε} {Γ : Ctx? α} {a : Term φ (Ty α)} {A : Ty α}
+  (D : Γ ⊢ a : A) [ha : HasEff e a] : E.HasEff e D.den := by
+  generalize ha = ha
+  induction D with
+  | iter =>
+    simp [den] at *
+    casesm* _ ∧ _
+    simp [*] at *
+    apply EffectfulCategory.HasEff.comp _ _ (hg := _)
+    apply EffectfulCategory.HasEff.comp _ _ (hg := _)
+    apply EffectfulCategory.HasEff.iterate _ (by assumption)
+  | _ =>
+    simp [den] at *
+    (try casesm* _ ∧ _)
+    (try simp [*] at *)
+    infer_instance
